theories/Var.v
@@ -1,0 +1,27 @@
+Require Import Unicode.Utf8.
+Require Import Vectors.Fin.
+Require Import Coq.Program.Equality.
+
+Set Implicit Arguments.
+
+Definition Ctx := nat.
+Definition Var := Fin.t.
+
+Module Ren.
+  Definition t (ψ1 ψ2 : Ctx) : Type :=
+    Var ψ1 → Var ψ2.
+
+  Program Definition cong {ψ1 ψ2} (ρ : t ψ1 ψ2) : t (S ψ1) (S ψ2) :=
+    fun x =>
+      match x with
+      | Fin.F1 => Fin.F1
+      | Fin.FS y => Fin.FS (ρ y)
+      end.
+
+  Program Fixpoint weak {ψ1} ψ2 : t ψ1 (ψ2 + ψ1) :=
+    match ψ2 with
+    | 0 => fun x => x
+    | S n => fun x => weak n (Fin.FS x)
+    end.
+
+End Ren.
